idea - 1:: using the concept of 
b/b = 1
b*(b^-1) = 1
(b*(b^-1))%m = 1%m;
(b%m*(b^-1)%m)%m = 1;
considering b^-1%m as INVERSE

(b%m * INVERSE) === 1;


```
int Solution::solve(int A, int B) {
    for(int i = 1; i < B; i++){
        if((A%B * i)%B == 1){
            return i;
        }
    }
}

```





idea - 2:: 

Fermat's little Theorm

b^-1%n = (b^m-2) % m

```

long long power(long long a, long long b, long long m) {
    long long result = 1;  // Initialize result
    a = a % m;  // Handle large numbers
    
    while (b > 0) {
        if (b & 1) {  // If b is odd, multiply a with result
            result = (result * a) % m;
        }
        a = (a * a) % m;  // Square a
        b >>= 1;  // Divide b by 2
    }
    
    return result;
}

int Solution::solve(int A, int B) {
    return (int)power(A,B - 2,B);
}


```
